code/ecdsap256sha2/Hacl.Impl.P256.DH.fst
@@ -1,0 +1,131 @@
+module Hacl.Impl.P256.DH
+
+open FStar.HyperStack.All
+open FStar.HyperStack
+module ST = FStar.HyperStack.ST
+
+open Lib.IntTypes
+open Lib.Buffer
+open Lib.ByteSequence
+
+open FStar.Mul
+open FStar.Math.Lemmas
+
+open Hacl.Hash.SHA2
+
+open Hacl.Spec.P256
+open Hacl.Spec.ECDSA
+open Hacl.Spec.P256.Lemmas
+open Hacl.Spec.P256.Definitions
+
+open Hacl.Spec.ECDSAP256.Definition
+
+open Hacl.Impl.LowLevel
+
+open Hacl.Impl.P256
+open Hacl.Impl.P256.Signature.Common
+
+
+#reset-options "--z3rlimit 300" 
+
+let ecp256dh_i result scalar = 
+  push_frame();
+    let tempBuffer = create (size 100) (u64 0) in 
+    let resultBuffer = create (size 12) (u64 0) in
+    let resultBufferX = sub resultBuffer (size 0) (size 4) in 
+    let resultBufferY = sub resultBuffer (size 4) (size 4) in 
+    
+    let resultX = sub result (size 0) (size 32) in 
+    let resultY = sub result (size 32) (size 32) in 
+
+    secretToPublic resultBuffer scalar tempBuffer; 
+    let flag = isPointAtInfinityPrivate resultBuffer in 
+  let h2 = ST.get() in
+    toUint8 resultBufferX resultX;
+      lemma_core_1 resultBufferX h2;
+      lemma_core_1 resultBufferY h2;
+    toUint8 resultBufferY resultY;
+  pop_frame(); 
+    flag
+
+
+val _ecp256dh_r: result: lbuffer uint64 (size 12) -> pubKey: lbuffer uint64 (size 8) -> scalar: lbuffer uint8 (size 32) -> 
+  Stack uint64 
+    (requires fun h -> live h result /\ live h pubKey /\ live h scalar /\ 
+      disjoint result pubKey /\ disjoint result scalar /\ disjoint pubKey scalar /\
+      Lib.ByteSequence.nat_from_bytes_le (as_seq h scalar) >= 1 /\
+      Lib.ByteSequence.nat_from_bytes_le (as_seq h scalar) < Hacl.Spec.ECDSAP256.Definition.prime_p256_order
+    )
+    (ensures fun h0 r h1 -> modifies (loc result) h0 h1 /\
+      (
+	let x, y = as_nat h0 (gsub pubKey (size 0) (size 4)), as_nat h0 (gsub pubKey (size 4) (size 4)) in 
+	let x3, y3, z3 = point_x_as_nat h1 result, point_y_as_nat h1 result, point_z_as_nat h1 result in 
+	let pointJacX, pointJacY, pointJacZ = toJacobianCoordinates (x, y) in 
+	if not (verifyQValidCurvePointSpec (pointJacX, pointJacY, pointJacZ)) then 
+	  uint_v r = maxint U64
+	else 
+	  let xN, yN, zN = scalar_multiplication (as_seq h0 scalar) (pointJacX, pointJacY, pointJacZ) in 
+	  xN == x3 /\ yN == y3 /\ zN == z3 /\
+	  (
+	    if isPointAtInfinity (xN, yN, zN) then 
+	      uint_v r = maxint U64
+	    else 
+	      uint_v r = 0
+	  )
+      )
+  )
+
+let _ecp256dh_r result pubKey scalar = 
+  push_frame();
+    let h0 = ST.get() in 
+    let tempBuffer = create (size 100) (u64 0) in 
+    let publicKeyBuffer = create (size 12) (u64 0) in 
+    bufferToJac pubKey publicKeyBuffer;
+    let publicKeyCorrect = verifyQValidCurvePoint publicKeyBuffer tempBuffer in 
+    if publicKeyCorrect = false then 
+      begin 
+	pop_frame();
+	u64 18446744073709551615
+      end
+    else
+      begin
+       scalarMultiplication publicKeyBuffer result scalar tempBuffer;
+       let flag = isPointAtInfinityPrivate result in 
+       pop_frame();
+       flag
+      end
+
+
+let ecp256dh_r result pubKey scalar = 
+  push_frame(); 
+    let h0 = ST.get() in 
+      let resultBufferFelem = create (size 12) (u64 0) in 
+	let resultBufferFelemX = sub resultBufferFelem (size 0) (size 4) in 
+	let resultBufferFelemY = sub resultBufferFelem (size 4) (size 4) in 
+	let resultX = sub result (size 0) (size 32) in 
+	let resultY = sub result (size 32) (size 32) in 
+      
+      let publicKeyAsFelem = create (size 8) (u64 0) in 
+	let publicKeyFelemX = sub publicKeyAsFelem (size 0) (size 4) in 
+	let publicKeyFelemY = sub publicKeyAsFelem (size 4) (size 4) in 
+	let pubKeyX = sub pubKey (size 0) (size 32) in 
+	let pubKeyY = sub pubKey (size 32) (size 32) in 
+
+      toUint64 pubKeyX publicKeyFelemX;
+      toUint64 pubKeyY publicKeyFelemY;
+      
+      let h1 = ST.get() in 
+	lemma_core_0 publicKeyFelemX h1;
+	Lib.ByteSequence.uints_from_bytes_le_nat_lemma #U64 #SEC #4 (as_seq h1 pubKeyX);
+	lemma_core_0 publicKeyFelemY h1;
+	Lib.ByteSequence.uints_from_bytes_le_nat_lemma #U64 #SEC #4 (as_seq h1 pubKeyY); 
+	
+	let flag = _ecp256dh_r resultBufferFelem publicKeyAsFelem scalar in 
+      let h2 = ST.get() in 	
+      toUint8 resultBufferFelemX resultX;
+	lemma_core_1 resultBufferFelemX h2;
+      toUint8 resultBufferFelemY resultY;
+	lemma_core_1 resultBufferFelemY h2;
+      pop_frame();
+      flag
+      
