code/ecdsap256sha2/Hacl.Impl.P256.DH.fsti
@@ -1,0 +1,72 @@
+module Hacl.Impl.P256.DH
+
+open FStar.HyperStack.All
+open FStar.HyperStack
+module ST = FStar.HyperStack.ST
+
+open Lib.IntTypes
+open Lib.Buffer
+open Lib.ByteSequence
+
+open FStar.Mul
+open FStar.Math.Lemmas
+
+open Hacl.Hash.SHA2
+
+open Hacl.Spec.P256
+open Hacl.Spec.ECDSA
+open Hacl.Spec.P256.Lemmas
+open Hacl.Spec.P256.Definitions
+
+open Hacl.Spec.ECDSAP256.Definition
+
+open Hacl.Impl.LowLevel
+
+open Hacl.Impl.P256
+open Hacl.Impl.P256.Signature.Common
+
+val ecp256dh_i: result: lbuffer uint8 (size 64) -> scalar: lbuffer uint8 (size 32) -> Stack uint64
+  (requires fun h -> live h result /\ live h scalar /\ disjoint result scalar /\
+    Lib.ByteSequence.nat_from_bytes_le (as_seq h scalar) >= 1 /\
+    Lib.ByteSequence.nat_from_bytes_le (as_seq h scalar) < Hacl.Spec.ECDSAP256.Definition.prime_p256_order
+  )
+  (ensures fun h0 r h1 -> modifies (loc result) h0 h1 /\
+    (
+      let xN, yN, zN = secret_to_public (as_seq h0 scalar) in 
+      let resultX = gsub result (size 0) (size 32) in 
+      let resultY = gsub result (size 32) (size 32) in 
+      if isPointAtInfinity (xN, yN, zN) then uint_v r = maxint U64 else uint_v r = 0 /\
+      Lib.ByteSequence.nat_from_bytes_le (as_seq h1 resultX) == xN /\
+      Lib.ByteSequence.nat_from_bytes_le (as_seq h1 resultY) == yN
+    )  
+  )
+
+
+val ecp256dh_r: result: lbuffer uint8 (size 64) -> pubKey: lbuffer uint8 (size 64) -> scalar: lbuffer uint8 (size 32) -> 
+  Stack uint64
+    (requires fun h -> 
+      live h result /\ live h pubKey /\ live h scalar /\
+      disjoint result pubKey /\ disjoint result scalar /\ disjoint pubKey scalar /\
+      Lib.ByteSequence.nat_from_bytes_le (as_seq h scalar) >= 1 /\
+      Lib.ByteSequence.nat_from_bytes_le (as_seq h scalar) < Hacl.Spec.ECDSAP256.Definition.prime_p256_order)
+    (ensures fun h0 flag h1 -> 
+      modifies (loc result) h0 h1 /\ 
+	(
+	  let pubKeyX, pubKeyY = gsub pubKey (size 0) (size 32), gsub pubKey (size 32) (size 32) in 
+	  let x, y = nat_from_bytes_le (as_seq h0 pubKeyX), nat_from_bytes_le (as_seq h0 pubKeyY) in 
+	  let resultX, resultY = gsub result (size 0) (size 32), gsub result (size 32) (size 32) in 
+	  let x3, y3 = nat_from_bytes_le (as_seq h1 resultX), nat_from_bytes_le (as_seq h1 resultY) in 
+	  let pointJacX, pointJacY, pointJacZ = toJacobianCoordinates (x, y) in 
+	  if not (verifyQValidCurvePointSpec (pointJacX, pointJacY, pointJacZ)) then 
+	    uint_v flag = maxint U64
+	  else 
+	    let xN, yN, zN = scalar_multiplication (as_seq h0 scalar) (pointJacX, pointJacY, pointJacZ) in 
+	    xN == x3 /\ yN == y3 /\
+	    (
+	      if isPointAtInfinity (xN, yN, zN) then 
+		uint_v flag = maxint U64
+	      else 
+		uint_v flag = 0
+	    )
+	)
+    )
