code/ecdsap256sha2/Hacl.Impl.P256.Signature.Common.fst
@@ -1,0 +1,263 @@
+module Hacl.Impl.P256.Signature.Common
+
+open FStar.HyperStack.All
+open FStar.HyperStack
+module ST = FStar.HyperStack.ST
+
+open Lib.IntTypes
+open Lib.ByteBuffer 
+open Lib.ByteSequence
+open Lib.Buffer 
+
+open Hacl.Spec.P256 
+open Hacl.Spec.P256.Definitions
+
+open Hacl.Spec.ECDSA
+open Hacl.Spec.ECDSAP256.Definition
+
+open Hacl.Impl.LowLevel
+open Hacl.Impl.ECDSA.MontgomeryMultiplication
+
+open Hacl.Impl.P256.LowLevel
+open Hacl.Impl.P256
+
+
+#set-options "--z3rlimit 100"
+
+val changeEndian: i: felem -> Stack unit 
+  (requires fun h -> live h i)
+  (ensures fun h0 _ h1 -> modifies1 i h0 h1 /\ as_seq h1 i == Hacl.Spec.ECDSA.changeEndian (as_seq h0 i)) 
+
+let changeEndian i = 
+  let zero = index i (size 0) in 
+  let one = index i (size 1) in 
+  let two = index i (size 2) in 
+  let three = index i (size 3) in 
+  upd i (size 0) three;
+  upd i (size 1) two; 
+  upd i (size 2) one;
+  upd i (size 3) zero
+
+
+val toUint64ChangeEndian: i: lbuffer uint8 (32ul) -> o: felem ->  Stack unit
+  (requires fun h -> live h i /\ live h o /\ disjoint i o)
+  (ensures fun h0 _ h1 -> 
+    modifies (loc o) h0 h1 /\ 
+    as_seq h1 o == Hacl.Spec.ECDSA.changeEndian(Lib.ByteSequence.uints_from_bytes_be #_ #_ #4 (as_seq h0 i))
+  )
+
+let toUint64ChangeEndian i o = 
+  Lib.ByteBuffer.uints_from_bytes_be o i;
+  changeEndian o
+
+
+val lemma_core_0: a: lbuffer uint64 (size 4) -> h: mem -> Lemma (nat_from_intseq_le (as_seq h a) == as_nat h a)
+
+let lemma_core_0 a h = 
+  let k = as_seq h a in 
+  let z = nat_from_intseq_le k in 
+    nat_from_intseq_le_slice_lemma k 1;
+    nat_from_intseq_le_lemma0 (Seq.slice k 0 1);
+  let k1 = Seq.slice k 1 4 in 
+    nat_from_intseq_le_slice_lemma #_ #_ #3 k1 1;
+    nat_from_intseq_le_lemma0 (Seq.slice k1 0 1);
+  let k2 = Seq.slice k1 1 3 in 
+    nat_from_intseq_le_slice_lemma #_ #_ #2 k2 1;
+    nat_from_intseq_le_lemma0 (Seq.slice k2 0 1);
+    nat_from_intseq_le_lemma0 (Seq.slice k2 1 2)
+
+
+val lemma_core_1: a: lbuffer uint64 (size 4) -> h: mem -> 
+  Lemma (nat_from_bytes_le (Lib.ByteSequence.uints_to_bytes_le (as_seq h a)) == as_nat h a)
+
+let lemma_core_1 a h= 
+  let open Lib.ByteSequence in 
+  lemma_core_0 a h;
+  lemma_nat_from_to_intseq_le_preserves_value #U64 #SEC 4 (as_seq h a);
+  let n = nat_from_intseq_le (as_seq h a) in 
+  uints_to_bytes_le_nat_lemma #U64 #SEC 4 n;
+  lemma_nat_to_from_bytes_le_preserves_value #SEC (uints_to_bytes_le #U64 #SEC #4 (as_seq h a)) 32 (as_nat h a)
+
+
+val bufferToJac: p: lbuffer uint64 (size 8) -> result: point -> Stack unit 
+  (requires fun h -> live h p /\ live h result /\ disjoint p result)
+  (ensures fun h0 _ h1 -> 
+    modifies (loc result) h0 h1 /\ as_nat h1 (gsub result (size 8) (size 4)) == 1 /\ 
+    (
+      let x = as_nat h0 (gsub p (size 0) (size 4)) in 
+      let y = as_nat h0 (gsub p (size 4) (size 4)) in 
+      let x3, y3, z3 = point_x_as_nat h1 result,  point_y_as_nat h1 result, point_z_as_nat h1 result in 
+      let pointJacX, pointJacY, pointJacZ = toJacobianCoordinates (x, y) in 
+      x3 == pointJacX /\ y3 == pointJacY /\ z3 == pointJacZ
+    )
+  )    
+    
+let bufferToJac p result = 
+  let partPoint = sub result (size 0) (size 8) in 
+  copy partPoint p;
+  upd result (size 8) (u64 1);
+  upd result (size 9) (u64 0);
+  upd result (size 10) (u64 0);
+  upd result (size 11) (u64 0)
+
+
+(* 
+  checks whether the coordinates are valid = 
+  all of them are less than prime 
+*) 
+
+
+(* checks whether the intefer f is between 1 and (n- 1) (incl).  *)
+(* [1, n - 1] <==> a > 0 /\ a < n) *)
+
+val isMoreThanZeroLessThanOrderMinusOne: f: felem -> Stack bool
+  (requires fun h -> live h f)
+  (ensures fun h0 result h1 -> modifies0 h0 h1 /\
+    (
+      if as_nat h0 f > 0 && as_nat h0 f < prime_p256_order then result == true else result == false
+    )  
+  )
+
+let isMoreThanZeroLessThanOrderMinusOne f = 
+  push_frame();
+    let tempBuffer = create (size 4) (u64 0) in 
+        recall_contents prime256order_buffer (Lib.Sequence.of_list p256_order_prime_list);
+    let carry = sub4_il f prime256order_buffer tempBuffer in  
+    let less = eq_u64_nCT carry (u64 1) in
+    let more = isZero_uint64_nCT f in 
+    let result = less && not more in 
+  pop_frame();  
+    result
+
+
+(* we require the coordinate to be in affine representation of jac coordinate *)
+val isCoordinateValid: p: point -> Stack bool 
+  (requires fun h -> live h p /\ point_z_as_nat h p == 1)
+  (ensures fun h0 r h1 -> 
+    modifies0 h0 h1  /\ 
+    (
+      if (point_x_as_nat h0 p < prime256 && point_y_as_nat h0 p < prime256 && point_z_as_nat h0 p < prime256) then r == true else r == false
+    )  
+  )
+
+let isCoordinateValid p = 
+  push_frame();
+    let tempBuffer = create (size 4) (u64 0) in 
+      recall_contents prime256_buffer (Lib.Sequence.of_list p256_prime_list);
+    let x = sub p (size 0) (size 4) in 
+    let y = sub p (size 4) (size 4) in 
+    
+    let carryX = sub4_il x prime256_buffer tempBuffer in
+    let carryY = sub4_il y prime256_buffer tempBuffer in 
+    
+    let lessX = eq_u64_nCT carryX (u64 1) in   
+    let lessY = eq_u64_nCT carryY (u64 1) in 
+
+    let r = lessX && lessY in 
+  pop_frame();
+    r  
+
+
+inline_for_extraction noextract
+val multByOrder: result: point ->  p: point -> tempBuffer: lbuffer uint64 (size 100) -> Stack unit 
+  (requires fun h -> 
+    live h result /\ live h p /\ live h tempBuffer /\
+    LowStar.Monotonic.Buffer.all_disjoint [loc result; loc p; loc tempBuffer] /\
+    point_x_as_nat h p < prime256 /\ 
+    point_y_as_nat h p < prime256 /\
+    point_z_as_nat h p < prime256
+  )
+  (ensures fun h0 _ h1 ->
+    modifies (loc result |+| loc p |+| loc tempBuffer) h0 h1 /\
+    (
+      let xN, yN, zN = scalar_multiplication prime_p256_order_seq (point_prime_to_coordinates (as_seq h0 p)) in 
+      let x3, y3, z3 = point_x_as_nat h1 result, point_y_as_nat h1 result, point_z_as_nat h1 result in 
+      x3 == xN /\ y3 == yN /\ z3 == zN 
+    ) 
+  )
+
+let multByOrder result p tempBuffer =
+  push_frame();
+      recall_contents order_buffer prime_p256_order_seq;
+    scalarMultiplication p result order_buffer tempBuffer;
+  pop_frame()
+
+
+inline_for_extraction noextract
+val multByOrder2: result: point ->  p: point -> tempBuffer: lbuffer uint64 (size 100) -> Stack unit 
+  (requires fun h -> 
+    live h result /\ live h p /\ live h tempBuffer /\
+    LowStar.Monotonic.Buffer.all_disjoint [loc result; loc p; loc tempBuffer] /\
+    point_x_as_nat h p < prime256 /\ 
+    point_y_as_nat h p < prime256 /\
+    point_z_as_nat h p < prime256
+  )
+  (ensures fun h0 _ h1  -> modifies (loc result |+| loc tempBuffer) h0 h1 /\
+    (
+      let xN, yN, zN = scalar_multiplication prime_p256_order_seq (point_prime_to_coordinates (as_seq h0 p)) in 
+      let x3, y3, z3 = point_x_as_nat h1 result, point_y_as_nat h1 result, point_z_as_nat h1 result in 
+      x3 == xN /\ y3 == yN /\ z3 == zN 
+    )
+  )
+
+let multByOrder2 result p tempBuffer = 
+  push_frame();
+    let pBuffer = create (size 12) (u64 0) in 
+    copy pBuffer p;
+    multByOrder result pBuffer tempBuffer;
+  pop_frame()  
+    
+
+(*checks whether the base point * order is point at infinity *)
+val isOrderCorrect: p: point -> tempBuffer: lbuffer uint64 (size 100) -> Stack bool
+  (requires fun h -> 
+    live h p /\ live h tempBuffer /\ 
+    disjoint p tempBuffer /\
+    point_x_as_nat h p < prime256 /\ 
+    point_y_as_nat h p < prime256 /\
+    point_z_as_nat h p < prime256
+  )
+  (ensures fun h0 r h1 -> 
+    modifies(loc tempBuffer) h0 h1 /\ 
+    (
+      let (xN, yN, zN) = scalar_multiplication prime_p256_order_seq (point_prime_to_coordinates (as_seq h0 p)) in 
+      if Hacl.Spec.P256.isPointAtInfinity (xN, yN, zN) then r == true else r == false
+    )
+  )
+
+let isOrderCorrect p tempBuffer = 
+  push_frame(); 
+    let multResult = create (size 12) (u64 0) in 
+    multByOrder2 multResult p tempBuffer;
+    let result = Hacl.Impl.P256.isPointAtInfinityPublic multResult in  
+   pop_frame();
+     result
+
+
+(*
+For Bob to authenticate Alice's signature, he must have a copy of her public-key curve point {\displaystyle Q_{A}} Q_{A}. Bob can verify {\displaystyle Q_{A}} Q_{A} is a valid curve point as follows:
+
+Check that {\displaystyle Q_{A}} Q_{A} is not equal to the identity element {\displaystyle O} O, and its coordinates are otherwise valid
+Check that {\displaystyle Q_{A}} Q_{A} lies on the curve
+Check that {\displaystyle n\times Q_{A}=O} n\times Q_{A}=O
+ *)
+ 
+val verifyQValidCurvePoint: pubKeyAsPoint: point -> tempBuffer: lbuffer uint64 (size 100) -> Stack bool
+  (requires fun h -> 
+    live h pubKeyAsPoint /\ live h tempBuffer /\
+    LowStar.Monotonic.Buffer.all_disjoint [loc pubKeyAsPoint; loc tempBuffer] /\
+    point_z_as_nat h pubKeyAsPoint == 1
+  )
+  (ensures fun h0 r h1 -> 
+    modifies (loc tempBuffer) h0 h1 /\ 
+    r == verifyQValidCurvePointSpec (point_prime_to_coordinates (as_seq h0 pubKeyAsPoint))
+  ) 
+
+let verifyQValidCurvePoint pubKeyAsPoint tempBuffer = 
+    let coordinatesValid = isCoordinateValid pubKeyAsPoint in 
+      if not coordinatesValid then false else
+    let belongsToCurve =  Hacl.Impl.P256.isPointOnCurvePublic pubKeyAsPoint in 
+    let orderCorrect = isOrderCorrect pubKeyAsPoint tempBuffer in 
+    if coordinatesValid && belongsToCurve && orderCorrect 
+      then true 
+    else false  
